

Apply

$$\text{Eqn (i)} - \frac{13}{3} \text{ Eqn (iv)}$$

$$13y - 27 = -19$$

$$13y + \frac{65}{3} = \frac{91}{3}$$

$$-27 - \frac{65}{3} = -19 - \frac{91}{3}$$

$$\Rightarrow \frac{-67 - 65}{3} = \frac{-57 - 91}{3}$$

$$\Rightarrow \frac{-71}{3} = \frac{-148}{3}$$

$$\therefore 7 = \frac{148}{71}$$

put 7 in Eqn (iv)

$$13y - 27 = -19$$

$$\Rightarrow 13y - 2 \times \frac{148}{71} = -19$$

$$\Rightarrow 13y = -19 + \frac{296}{71}$$

$$\Rightarrow 13y = \frac{-1349 + 296}{71}$$

$$\Rightarrow y = \frac{-1053}{923}$$

$$\therefore y = \frac{-81}{71}$$

Put y & z in eqn (i)

$$x + 4y - z = -5$$

$$\Rightarrow x + 4 \times \left(\frac{-81}{71} \right) - \frac{148}{71} = -5$$

$$\Rightarrow x = -5 + \frac{324}{71} + \frac{148}{71}$$

$$\therefore x = \frac{117}{71}$$

Here,

$$x = \frac{117}{71}, y = \frac{-81}{71}, z = \frac{148}{71}$$

(Signature)

2. Gauss's Seidel iterative method.

Q. $\begin{cases} 20x + y - 2z = 17 \\ 3x + 20y - z = -18 \\ 2x - 3y + 20z = 25 \end{cases}$

Firstly select x, y, z

$$x = \frac{1}{20} (17 - y + 2z) \quad \text{--- (i)}$$

$$y = \frac{1}{20} (-18 - 3x + z) \quad \text{--- (ii)}$$

$$z = \frac{1}{20} (25 - 2x + 3y) \quad \text{--- (iii)}$$

Iteration 1.

Let $y=0$, $z=0$ put in equation (i)

$$x^{(1)} = \frac{1}{20} (17 - 0 + 0) = \frac{1}{20} \times 17 = 0.85$$

Now,

$x^{(1)} = 0.85$, $z=0$ put in eqn (ii)

$$y^{(1)} = \frac{1}{20} (-18 - 3 \times 0.85 + 0)$$

$$\Rightarrow y^{(1)} = \frac{1}{20} \times (-20.55)$$

$$\therefore y^{(1)} = -1.0275$$

Now,

$x^{(1)} = 0.85$, $y^{(1)} = -1.0275$

$$z^{(1)} = \frac{1}{20} [25 - 2 \times 0.85 + 3 \times (-1.0275)]$$

$$\Rightarrow z^{(1)} = \frac{1}{20} \times 20.2175$$

$$\therefore z^{(1)} = 1.010875 \approx 1.0109$$

Iteration 2

$x^{(1)} = 0.85$, $y^{(1)} = -1.0275$, $z^{(1)} = 1.0109$

put in eqn (i)

$$x^{(2)} = \frac{1}{20} (17 + 1.0275 + 2 \times 1.0109)$$

$$\Rightarrow x^{(2)} = \frac{1}{20} \times 20.0493$$

$$\therefore x^{(2)} = 1.0025$$

Now,

$$x^{(2)} = 1.0025, \quad z^{(1)} = 1.0109$$

Put in eqn (ii)

$$y^{(2)} = \frac{1}{20} (-18 - 3 \times 1.0025 + 1.0109)$$

$$\Rightarrow y^{(2)} = \frac{1}{20} \times (-19.9966)$$

$$\therefore y^{(2)} = -0.9998$$

Now,

$$x^{(2)} = 1.0025, \quad y^{(2)} = -0.9998$$

Put in eqn (iii)

$$z^{(2)} = \frac{1}{20} (25 - 2 \times 1.0025 - 3 \times -0.9998)$$

$$\Rightarrow z^{(2)} = \frac{1}{20} \times 19.9956$$

$$\therefore z^{(2)} = 0.99978$$

Iteration

$$x^{(2)} = 1.0025, \quad y^{(2)} = -0.9998, \quad z^{(2)} = 0.9998$$

Put in eqn (i)

$$x^{(3)} = \frac{1}{20} (17 + 0.9998 + 2 \times 0.9998)$$

$$\Rightarrow x^{(3)} = \frac{1}{20} \times 19.9994$$

$$\therefore x^{(3)} = 0.99997$$

Now,

$$z^{(2)} = 0.9997, \quad y^{(2)} = 0.9998$$

Put the eqn (ii)

$$y^{(3)} = \frac{1}{20} (-18 - 3 \times 0.9997 + 0.9998)$$

$$\Rightarrow y^{(3)} = \frac{1}{20} \times (-19.9993)$$

$$\therefore y^{(3)} = -0.9996$$

Now,

$$z^{(3)} = 0.99997, \quad y^{(3)} = -0.99996$$

Put in eqn (iii)

$$z^{(4)} = \frac{1}{20} (25 + 2 \times 0.99997 - 3 \times 0.99996)$$

$$\Rightarrow z^{(4)} = \frac{1}{20} \times 10.00018$$

$$\therefore z^{(4)} = 1.000009$$

Here,

$$\begin{matrix} x = 1 \\ y = -1 \\ z = 1 \end{matrix}$$

